theories/case_studies/multiuser_kvs/kvs_spec_erase_safe.v
@@ -102,7 +102,7 @@ Section KVS_spec_erase.
 
     (* Either the map key is already allocated, or it is not *)
     destruct (m !! nkey)  as [ w | ] eqn:Hnkey.
-    - iApply KVS_erase_spec_in; last iFrame "∗#"; eauto.
+    - iApply KVS_erase_spec_in_layer_2; last iFrame "∗#"; eauto.
       iNext.
       iIntros "(Hna & HPC & Hgcp & Hcra & Hca0 & Hca1 & Hct1 & Hct2 & Hctp & Hcnull
                 & Ha & Hm)".
@@ -116,7 +116,7 @@ Section KVS_spec_erase.
 
       iApply "Hpost"; iFrame.
 
-    - iApply KVS_erase_spec_notin; last iFrame "∗#"; eauto.
+    - iApply KVS_erase_spec_notin_layer_2; last iFrame "∗#"; eauto.
       iNext.
       iIntros "(Hna & HPC & Hgcp & Hcra & Hca0 & Hca1 & Hct1 & Hct2 & Hctp & Hcnull
                 & Ha & Hm)".
