theories/case_studies/multiuser_kvs/kvs_spec_read.v
@@ -19,7 +19,7 @@ Section KVS_spec_read.
 
   (*** KVS READ: Read key in the KVS *)
 
-  Lemma KVS_read_spec_in_pre
+  Lemma KVS_read_spec_in_layer_1
     (pc_b pc_e pc_a : Addr)
     (cgp_b cgp_e : Addr)
     (wret : Word)
@@ -149,7 +149,7 @@ Section KVS_spec_read.
     iApply "Hpost"; iFrame "∗%".
   Qed.
 
-  Lemma KVS_read_spec_in
+  Lemma KVS_read_spec_in_layer_2
     (wret wca2 : Word)
     (user_key : user_key_t) (nkey : map_key_t) (l_user_key : Locality) (user_key_addr : Addr)
     (m : kvs_user_map) (w : Word)
@@ -220,7 +220,7 @@ Section KVS_spec_read.
     rewrite /kvs_service_instrs.
     focus_block_nochangePC 1 "Hcode" as a_read Ha_read "Hcode" "Hcont"; iHide "Hcont" as hcont.
     assert (a_read = kvs_read_pcc_addr) as -> by (rewrite /kvs_read_pcc_addr ; cbn in * ; solve_addr+Hcode_continuous HKVS_pcc_b' Ha_read).
-    iApply (KVS_read_spec_in_pre with "[- $HPC]"); last iFrame; eauto.
+    iApply (KVS_read_spec_in_layer_1 with "[- $HPC]"); last iFrame; eauto.
     iNext; iIntros "(HPC & Hcgp & Hcra & Hca0 & Hca1 & Hctp & Hct1 & Hct2
               & Hcnull & Hcode & Ha_unsealing & Ha_user_key & Hlkvs_frag & HKVS & Hm)".
     subst hcont; unfocus_block "Hcode" "Hcont" as "Hcode".
@@ -234,9 +234,81 @@ Section KVS_spec_read.
     iApply "Hpost"; iFrame.
   Qed.
 
+  Lemma KVS_read_spec_in
+    (wret wca2 : Word)
+    (user_key : user_key_t) (nkey : map_key_t) (l_user_key : Locality) (user_key_addr : Addr)
+    (w : Word)
+    (E : coPset)
+    :
+    let fkey := (kvs_full_key user_key nkey) in
+
+    ↑Nkvs ⊆ E ->
+    ↑Nkvs_user.@user_key ⊆ E ->
+
+    is_uint16 nkey ->
+    withinBounds user_key_addr (user_key_addr ^+ 1)%a user_key_addr = true ->
+
+    ( na_inv cerise_nais Nkvs kvs_inv ∗
+      na_inv cerise_nais (Nkvs_user.@user_key) (logical_user_kvs_inv user_key) ∗
+      na_own cerise_nais E ∗
+
+      (* initial register file *)
+      PC ↦ᵣ WCap RX Global KVS_pcc_b KVS_pcc_e kvs_read_pcc_addr ∗
+      cgp ↦ᵣ WCap RW Global KVS_cgp_b KVS_cgp_e KVS_cgp_b ∗
+      cra ↦ᵣ wret ∗
+      ca0 ↦ᵣ kvs_user_seal_key l_user_key user_key_addr ∗ (* Sealed User Key *)
+      ca1 ↦ᵣ WInt nkey ∗ (* Key to read *)
+      ct1 ↦ᵣ - ∗ (* scratch *)
+      ct2 ↦ᵣ - ∗ (* scratch *)
+      ctp ↦ᵣ - ∗ (* scratch *)
+      cnull ↦ᵣ - ∗
+
+      user_key_addr ↦ₐ WInt user_key ∗
+
+      ▷ (user_key, nkey) ↦(KVS) w ∗
+
+      ▷ (na_own cerise_nais E ∗
+         PC ↦ᵣ updatePcPerm wret ∗
+         cgp ↦ᵣ - ∗
+         cra ↦ᵣ - ∗
+         ca0 ↦ᵣ WInt ASM_TRUE ∗ (* TRUE: the key exists in the map *)
+         ca1 ↦ᵣ w ∗ (* result of the read *)
+         ct1 ↦ᵣ - ∗ (* scratch *)
+         ct2 ↦ᵣ - ∗ (* scratch *)
+         ctp ↦ᵣ - ∗ (* scratch *)
+         cnull ↦ᵣ - ∗
+
+         user_key_addr ↦ₐ WInt user_key ∗
+
+         (user_key, nkey) ↦(KVS) w
+
+         -∗ WP Seq (Instr Executable) {{ v, ⌜v = HaltedV⌝ → na_own cerise_nais ⊤ }}
+        )
+      ⊢ WP Seq (Instr Executable) {{ v, ⌜v = HaltedV⌝ → na_own cerise_nais ⊤ }})%I.
+  Proof.
+    intros fkey.
+    iIntros (Hnkvs_E Hnkvs_user_E His_uint16_nkey Hbounds_a_user_key)
+      "(#Hkvs_inv & #Hkvs_user_inv & Hna & HPC & Hcgp & Hcra & Hca0 & Hca1 & Hctp & Hct1 & Hct2 & Hcnull
+      & Ha_user_key & >Hk & Hpost)".
+    iMod (na_inv_acc with "Hkvs_user_inv Hna")
+      as "( (%ukvs & >Hukvs_auth & (%m & Hm & >%Hsync)) & Hna & Hkvs_user_inv_close)"; eauto.
+
+    iDestruct (kvs_user_kvs_valid with "Hukvs_auth Hk") as "%Hk".
+    opose proof (kvs_synced_logical_user_kvs_Some _ _ _ _ _ Hk) as Hm_kvs; eauto.
+
+    iApply (KVS_read_spec_in_layer_2 with "[- $HPC]"); last iFrame "∗#"; eauto.
+    { pose proof Nkvs_namespaces_disjoint as (?&?&?&?&?&?); solve_ndisj. }
+    iNext; iIntros "(Hna & HPC & Hcgp & Hcra & Hca0 & Hca1 & Hctp & Hct1 & Hct2 & Hcnull
+              & Ha_user_key & Hm)".
+
+    iMod ("Hkvs_user_inv_close" with "[$Hna $Hukvs_auth $Hm]") as "Hna" ; auto.
+
+    iApply "Hpost"; iFrame; done.
+  Qed.
+
   (*** KVS READ: Read key not in the KVS *)
 
-  Lemma KVS_read_spec_notin_pre
+  Lemma KVS_read_spec_notin_layer_1
     (pc_b pc_e pc_a : Addr)
     (cgp_b cgp_e : Addr)
     (wret : Word)
@@ -384,7 +456,7 @@ Section KVS_spec_read.
         iApply "Hpost"; iFrame "∗%"; done.
   Qed.
 
-  Lemma KVS_read_spec_notin
+  Lemma KVS_read_spec_notin_layer_2
     (wret wca2 : Word)
     (user_key : user_key_t) (nkey : map_key_t) (l_user_key : Locality) (user_key_addr : Addr)
     (m : kvs_user_map)
@@ -452,7 +524,7 @@ Section KVS_spec_read.
     rewrite /kvs_service_instrs.
     focus_block_nochangePC 1 "Hcode" as a_read Ha_read "Hcode" "Hcont"; iHide "Hcont" as hcont.
     assert (a_read = kvs_read_pcc_addr) as -> by (rewrite /kvs_read_pcc_addr ; cbn in * ; solve_addr+Hcode_continuous HKVS_pcc_b' Ha_read).
-    iApply (KVS_read_spec_notin_pre with "[- $HPC]"); last iFrame; eauto.
+    iApply (KVS_read_spec_notin_layer_1 with "[- $HPC]"); last iFrame; eauto.
     iNext; iIntros "(HPC & Hcgp & Hcra & Hca0 & Hca1 & Hctp & Hct1 & Hct2
               & Hcnull & Hcode & Ha_unsealing & Ha_user_key & Hlkvs_frag & HKVS & Hm)".
     subst hcont; unfocus_block "Hcode" "Hcont" as "Hcode".
@@ -464,6 +536,72 @@ Section KVS_spec_read.
       rewrite /region_pointsto finz_seq_between_empty; auto; solve_addr+.
     }
     iApply "Hpost"; iFrame.
+  Qed.
+
+  Lemma KVS_read_spec_notin
+    (wret wca2 : Word)
+    (user_key : user_key_t) (nkey : map_key_t) (l_user_key : Locality) (user_key_addr : Addr)
+    (E : coPset)
+    :
+
+    ↑Nkvs ⊆ E ->
+    ↑Nkvs_user.@user_key ⊆ E ->
+
+    is_uint16 nkey ->
+    withinBounds user_key_addr (user_key_addr ^+ 1)%a user_key_addr = true ->
+
+    ( na_inv cerise_nais Nkvs kvs_inv ∗
+      na_inv cerise_nais (Nkvs_user.@user_key) (logical_user_kvs_inv user_key) ∗
+      na_own cerise_nais E ∗
+
+      (* initial register file *)
+      PC ↦ᵣ WCap RX Global KVS_pcc_b KVS_pcc_e kvs_read_pcc_addr ∗
+      cgp ↦ᵣ WCap RW Global KVS_cgp_b KVS_cgp_e KVS_cgp_b ∗
+      cra ↦ᵣ wret ∗
+      ca0 ↦ᵣ kvs_user_seal_key l_user_key user_key_addr ∗ (* Sealed User Key *)
+      ca1 ↦ᵣ WInt nkey ∗ (* Key to read *)
+      ct1 ↦ᵣ - ∗ (* scratch *)
+      ct2 ↦ᵣ - ∗ (* scratch *)
+      ctp ↦ᵣ - ∗ (* scratch *)
+      cnull ↦ᵣ - ∗
+
+      user_key_addr ↦ₐ WInt user_key ∗
+
+      ▷ (user_key, nkey) ↦(KVS) ⊥ ∗
+
+      ▷ (na_own cerise_nais E ∗
+         PC ↦ᵣ updatePcPerm wret ∗
+         cgp ↦ᵣ - ∗
+         cra ↦ᵣ - ∗
+         ca0 ↦ᵣ WInt ASM_FALSE ∗ (* FALSE: the key does not exist in the map *)
+         ca1 ↦ᵣ WInt 0 ∗ (* Dummy value *)
+         ct1 ↦ᵣ - ∗ (* scratch *)
+         ct2 ↦ᵣ - ∗ (* scratch *)
+         ctp ↦ᵣ - ∗ (* scratch *)
+         cnull ↦ᵣ - ∗
+         user_key_addr ↦ₐ WInt user_key ∗
+         (user_key, nkey) ↦(KVS) ⊥
+         -∗ WP Seq (Instr Executable) {{ v, ⌜v = HaltedV⌝ → na_own cerise_nais ⊤ }}
+        )
+      ⊢ WP Seq (Instr Executable) {{ v, ⌜v = HaltedV⌝ → na_own cerise_nais ⊤ }})%I.
+  Proof.
+    iIntros (Hnkvs_E Hnkvs_user_E His_uint16_nkey Hbounds_a_user_key)
+      "(#Hkvs_inv & #Hkvs_user_inv & Hna & HPC & Hcgp & Hcra & Hca0 & Hca1 & Hctp & Hct1 & Hct2 & Hcnull
+      & Ha_user_key & >Hk & Hpost)".
+    iMod (na_inv_acc with "Hkvs_user_inv Hna")
+      as "( (%ukvs & >Hukvs_auth & (%m & Hm & >%Hsync)) & Hna & Hkvs_user_inv_close)"; eauto.
+
+    iDestruct (kvs_user_kvs_valid with "Hukvs_auth Hk") as "%Hk".
+    opose proof (kvs_synced_logical_user_kvs_None _ _ _ _ Hk) as Hm_kvs; eauto.
+
+    iApply (KVS_read_spec_notin_layer_2 with "[- $HPC]"); last iFrame "∗#"; eauto.
+    { pose proof Nkvs_namespaces_disjoint as (?&?&?&?&?&?); solve_ndisj. }
+    iNext; iIntros "(Hna & HPC & Hcgp & Hcra & Hca0 & Hca1 & Hctp & Hct1 & Hct2 & Hcnull
+              & Ha_user_key & Hm)".
+
+    iMod ("Hkvs_user_inv_close" with "[$Hna $Hukvs_auth $Hm]") as "Hna" ; auto.
+
+    iApply "Hpost"; iFrame; done.
   Qed.
 
   (*** KVS READ: Ill-formed inputs *)
